Monad.v
@@ -3,61 +3,229 @@ Require Import FunctionalExtensionality.
 
 Generalizable All Variables.
 
-Definition State (s a : Type) := s -> (a * s).
+Class Functor (f : Set -> Set) := {
+  fmap : forall {a b : Set}, (a -> b) -> f a -> f b;
 
-Definition get  {s}     : State s s := fun i => (i, i).
-Definition gets {s a} f : State s a := fun s => (f s, s).
-Definition put  {s} x   : State s unit := fun _ => (tt, x).
-
-Definition modify {s} (f : s -> s) : State s unit := fun i => (tt, f i).
-
-Class Functor (f : Type -> Type) := {
-  fmap : forall {a b}, (a -> b) -> f a -> f b;
-
-  fun_id   : forall a, fmap (@id a) =1 id;
-  fun_comp : forall a b c f g, @fmap b c f \o @fmap a b g =1 @fmap a c (f \o g)
+  fmap_id   : forall a : Set, fmap (@id a) =1 id;
+  fmap_comp : forall (a b c : Set) (f : b -> c) (g : a -> b),
+    fmap f \o fmap g =1 fmap (f \o g)
 }.
 
 Arguments fmap {f _ a b} _ x.
 
+Notation "f $ x" := (f x) (at level 60, right associativity, only parsing).
+
+Definition apply `(f : a -> b) (x : a) : b := f x.
+
+Definition compose {a b c : Set} (f : b -> c) (g : a -> b) : a -> c := f \o g.
+
+Definition first `(f : a -> b) `(x : a * z) : b * z :=
+  match x with (a, z) => (f a, z) end.
+
+Lemma first_id : forall a z, first (a:=a) (b:=a) (z:=z) id = id.
+Proof.
+  rewrite /first.
+  move=> a z.
+  extensionality x.
+  by case: x.
+Qed.
+
+Definition second `(f : a -> b) `(x : z * a) : z * b :=
+  match x with (z, b) => (z, f b) end.
+
+Definition curry `(f : a -> b -> c) (x : (a * b)) : c :=
+  match x with (a, b) => f a b end.
+
+Lemma curry_apply_first : forall a b c d (f : (a -> b) -> c -> d),
+  curry apply \o first (a:=a -> b) (b:=c -> d) (z:=c) f = curry f.
+Proof.
+  move=> a b c d f.
+  extensionality x.
+  by case: x.
+Qed.
+
+Notation "f <$> x" :=
+  (fmap f x) (at level 28, left associativity, only parsing).
+Notation "x <&> f" :=
+  (fmap f x) (at level 28, left associativity, only parsing).
+
+Corollary fmap_id_x `{Functor f} : forall (a : Set) x, fmap (@id a) x = x.
+Proof. exact: fmap_id. Qed.
+
+Corollary fmap_comp_x `{Functor F} :
+  forall (a b c : Set) (f : b -> c) (g : a -> b) x,
+  fmap f (fmap g x) = fmap (fun y => f (g y)) x.
+Proof. exact: fmap_comp. Qed.
+
+Ltac recomp :=
+  repeat match goal with
+    | [ |- ?F (?G ?X) = _ ] =>
+        replace (F (G X)) with ((F \o G) X); last by rewrite /funcomp
+    | [ |- _ = ?F (?G ?X) ] =>
+        replace (F (G X)) with ((F \o G) X); last by rewrite /funcomp
+    end.
+
+Corollary fmap_docomp `{Functor F} :
+  forall (a b c : Set) (f : b -> c) (g : a -> b) x,
+  fmap f (fmap g x) = (fmap f \o fmap g) x.
+Proof. by rewrite /funcomp. Qed.
+
 Reserved Notation "f <*> g" (at level 28, left associativity).
 
-Class Applicative (f : Type -> Type) := {
+Class Applicative (f : Set -> Set) := {
   is_functor :> Functor f;
 
-  pure : forall {a}, a -> f a;
-  ap   : forall {a b}, f (a -> b) -> f a -> f b
+  pure : forall {a : Set}, a -> f a;
+  ap   : forall {a b : Set}, f (a -> b) -> f a -> f b
     where "f <*> g" := (ap f g);
 
-  ap_id : forall a, ap (pure (@id a)) =1 id;
-  ap_comp : forall a b c (v : f (a -> b)) (u : f (b -> c)) (w : f a),
-    pure (funcomp tt) <*> u <*> v <*> w = u <*> (v <*> w);
-  ap_homo : forall a b (x : a) (f : a -> b), pure f <*> pure x = pure (f x);
-  ap_interchange : forall a b (y : a) (u : f (a -> b)),
+  ap_id : forall a : Set, ap (pure (@id a)) =1 id;
+  ap_comp : forall (a b c : Set) (v : f (a -> b)) (u : f (b -> c)) (w : f a),
+    pure compose <*> u <*> v <*> w = u <*> (v <*> w);
+  ap_homo : forall (a b : Set) (x : a) (f : a -> b),
+    pure f <*> pure x = pure (f x);
+  ap_interchange : forall (a b : Set) (y : a) (u : f (a -> b)),
     u <*> pure y = pure (fun f => f y) <*> u;
 
-  ap_fmap : forall a b (f : a -> b), ap (pure f) =1 @fmap _ is_functor _ _ f
+  ap_fmap : forall (a b : Set) (f : a -> b),
+    ap (pure f) =1 @fmap _ is_functor _ _ f
 }.
 
 Arguments pure {f _ _} _.
 Arguments ap   {f _ _ _} _ x.
 
-Class Monad (m : Type -> Type) := {
+Notation "f <*> g" := (ap f g) (at level 28, left associativity).
+
+Corollary fmap_pure `{Applicative m} : forall (a b : Set) (f : a -> b),
+  fmap f \o pure =1 pure \o f.
+Proof.
+  move=> a b f x.
+  rewrite /funcomp -ap_fmap.
+  exact: ap_homo.
+Qed.
+
+Corollary fmap_pure_x `{Applicative m} : forall (a b : Set) (f : a -> b) x,
+  fmap f (pure x) = pure (f x).
+Proof. exact: fmap_pure. Qed.
+
+Class Monad (m : Set -> Set) := {
   is_applicative :> Applicative m;
 
-  join : forall {a}, m (m a) -> m a;
+  join : forall {a : Set}, m (m a) -> m a;
 
-  join_fmap_join : forall a, join \o fmap (@join a) =1 join \o join;
-  join_fmap_pure : forall a, join \o fmap (pure (a:=a)) =1 id;
-  join_pure      : forall a, join \o pure =1 @id (m a);
-  join_fmap_fmap : forall a b (f : a -> b),
+  join_fmap_join : forall a : Set, join \o fmap (@join a) =1 join \o join;
+  join_fmap_pure : forall a : Set, join \o fmap (pure (a:=a)) =1 id;
+  join_pure      : forall a : Set, join \o pure =1 @id (m a);
+  join_fmap_fmap : forall (a b : Set) (f : a -> b),
     join \o fmap (fmap f) =1 fmap f \o join
 }.
 
 Arguments join {m _ _} _.
 
-Program Instance State_Functor {S} : Functor (State S) := {
-  fmap := fun A B f (x : State S A) => fun st => match x st with
+Corollary join_fmap_join_x `{Monad m} : forall a x,
+  join (fmap (join (a:=a)) x) = join (join x).
+Proof. exact: join_fmap_join. Qed.
+
+Corollary join_fmap_pure_x `{Monad m} : forall a x,
+  join (fmap (pure (a:=a)) x) = x.
+Proof. exact: join_fmap_pure. Qed.
+
+Corollary join_pure_x `{Monad m} : forall a x,
+  join (pure x) = @id (m a) x.
+Proof. exact: join_pure. Qed.
+
+Corollary join_fmap_fmap_x `{Monad m} : forall (a b : Set) (f : a -> b) x,
+    join (fmap (fmap f) x) = fmap f (join x).
+Proof. exact: join_fmap_fmap. Qed.
+
+Definition liftA2 `{Applicative m} {A B C : Set}
+  (f : A -> B -> C) (x : m A) (y : m B) : m C := ap (fmap f x) y.
+
+Definition const {A B : Set} (x : B) : A -> B := fun _ => x.
+
+Definition chain `{Applicative m} {X Y} (a : m X) (b : m Y) : m Y :=
+  fmap const b <*> a.
+
+Notation "a >> b" := (chain a b) (at level 25, left associativity).
+
+Definition bind `{Monad m} {X Y : Set} (f : (X -> m Y)) : m X -> m Y :=
+  join \o fmap f.
+
+Notation "m >>= f" := (bind f m) (at level 25, left associativity).
+
+Notation "X <-- A ;; B" := (A >>= (fun X => B))
+  (right associativity, at level 84, A at next level).
+
+Notation "A ;; B" := (_ <-- A ;; B)
+  (right associativity, at level 84).
+
+Fixpoint mapM `{Applicative m} {A B} (f : A -> m B) (l : list A) :
+  m (list B) :=
+  match l with
+  | nil => pure nil
+  | cons x xs => liftA2 (@cons _) (f x) (mapM f xs)
+  end.
+
+Definition forM `{Applicative m} {A B} (l : list A) (f : A -> m B) :
+  m (list B) := mapM f l.
+
+Fixpoint mapM_ `{Applicative m} {A B} (f : A -> m B) (l : list A) : m unit :=
+  match l with
+  | nil => pure tt
+  | cons x xs => f x >> mapM_ f xs
+  end.
+
+Definition forM_ `{Applicative m} {A B} (l : list A) (f : A -> m B) : m unit :=
+  mapM_ f l.
+
+Definition foldM `{Monad m} {A B : Set}
+  (f : A -> B -> m A) (s : A) (l : list B) : m A :=
+  let fix go xs z :=
+      match xs with
+        | nil => pure z
+        | cons y ys => f z y >>= go ys
+      end in
+  go l s.
+
+Definition forFoldM `{Monad m} {A B : Set}
+  (s : A) (l : list B) (f : A -> B -> m A) : m A := foldM f s l.
+
+Definition foldrM `{Monad m} {A B : Set}
+  (f : B -> A -> m A) (s : A) (l : list B) : m A :=
+  let fix go xs z :=
+      match xs with
+        | nil => pure z
+        | cons y ys => go ys z >>= f y
+      end in
+  go l s.
+
+Definition forFoldrM `{Monad m} {A B : Set}
+  (s : A) (l : list B) (f : B -> A -> m A) : m A := foldrM f s l.
+
+Fixpoint concat {A : Set} (l : list (list A)) : list A :=
+  match l with
+  | nil => nil
+  | cons x xs => x ++ concat xs
+  end.
+
+Definition concatMapM `{Applicative m} {A B : Set}
+  (f : A -> m (list B)) (l : list A) : m (list B) :=
+  fmap (concat) (mapM f l).
+
+(******************************************************************************
+ * The State Monad
+ *)
+
+Definition State (s a : Set) := s -> (a * s).
+
+Definition get  {s : Set}     : State s s := fun i => (i, i).
+Definition gets {s a : Set} f : State s a := fun s => (f s, s).
+Definition put  {s : Set} x   : State s unit := fun _ => (tt, x).
+
+Definition modify {s : Set} (f : s -> s) : State s unit := fun i => (tt, f i).
+
+Program Instance State_Functor {s : Set} : Functor (State s) := {
+  fmap := fun A B f (x : State s A) => fun st => match x st with
     | (a,st') => (f a, st')
     end
 }.
@@ -72,7 +240,7 @@ Obligation 2.
   by case: (x st).
 Qed.
 
-Program Instance State_Applicative {S} : Applicative (State S) := {
+Program Instance State_Applicative {s : Set} : Applicative (State s) := {
   pure := fun _ x => fun st => (x, st);
 
   ap := fun _ _ f x => fun st => match f st with
@@ -94,7 +262,7 @@ Obligation 2.
   by case: (w st'').
 Qed.
 
-Program Instance State_Monad {S} : Monad (State S) := {
+Program Instance State_Monad {s : Set} : Monad (State s) := {
   join := fun _ x => fun st => match x st with
     | (y, st') => match y st' with
       | (a, st'') => (a, st'')
@@ -129,69 +297,155 @@ Obligation 4.
   by case: (f' st') => f'' st''.
 Qed.
 
-Definition bind `{Monad m} {X Y} (f : (X -> m Y)) (x : m X) : m Y :=
-  join (fmap f x).
+(******************************************************************************
+ * The StateT Monad transformer
+ *)
 
-Definition liftA2 `{Monad m} {A B C}
-  (f : A -> B -> C) (x : m A) (y : m B) : m C := ap (fmap f x) y.
 
-Notation "m >>= f" := (bind f m) (at level 25, left associativity).
+Definition StateT (s : Set) (m : Set -> Set) (a : Set):=
+  s -> m (a * s)%type.
 
-Notation "X <-- A ;; B" := (A >>= (fun X => B))
-  (right associativity, at level 84, A at next level).
+Definition getT  `{Applicative m} {s : Set}     : StateT s m s :=
+  fun i => pure (i, i).
+Definition getsT `{Applicative m} {s a : Set} f : StateT s m a :=
+  fun s => pure (f s, s).
+Definition putT  `{Applicative m} {s : Set} x   : StateT s m unit :=
+  fun _ => pure (tt, x).
 
-Notation "A ;; B" := (_ <-- A ;; B)
-  (right associativity, at level 84).
+Definition modifyT `{Applicative m} {s : Set} (f : s -> s) : StateT s m unit :=
+  fun i => pure (tt, f i).
 
-Fixpoint mapM `{Monad m} {A B} (f : A -> m B) (l : list A) :
-  m (list B) :=
-  match l with
-  | nil => pure nil
-  | cons x xs => liftA2 (@cons _) (f x) (mapM f xs)
-  end.
+Program Instance StateT_Functor {s} `{Functor m} : Functor (StateT s m) := {
+  fmap := fun A B f (x : StateT s m A) => fun st =>
+    x st <&> first f
+}.
+Obligation 1.
+  move=> x.
+  extensionality st.
+  rewrite first_id.
+  replace (fun z : a * s => (z.1, z.2)) with (@id (a * s)%type); last first.
+    by extensionality z; case z.
+  by rewrite fmap_id.
+Qed.
+Obligation 2.
+  rewrite /funcomp => x.
+  extensionality st.
+  rewrite fmap_comp_x /first.
+  f_equal.
+  extensionality y.
+  by case: y.
+Qed.
 
-Definition forM `{Monad m} {A B} (l : list A) (f : A -> m B) : m (list B) :=
-  mapM f l.
+Definition StateT_ap `{Monad m} {s : Set} {a b : Set}
+  (f : StateT s m (a -> b)) (x : StateT s m a) : StateT s m b := fun st =>
+  join $ f st <&> fun z => match z with
+    | (f', st') => x st' <&> first f'
+    end.
 
-Fixpoint mapM_ `{Monad m} {A B} (f : A -> m B) (l : list A) : m unit :=
-  match l with
-  | nil => pure tt
-  | cons x xs => f x >>= fun _ => mapM_ f xs
-  end.
+Program Instance StateT_Applicative `{Monad m} {s : Set} :
+  Applicative (StateT s m) := {
+  pure := fun _ x => fun st => pure (x, st);
+  ap   := @StateT_ap m _ s
+}.
+Obligation 1.
+  move=> x.
+  extensionality st.
+  rewrite /StateT_ap fmap_pure_x join_pure_x.
+  set f := (X in fmap X).
+  replace f with (@id (a * s)%type); last first.
+    extensionality z.
+    by case: z.
+  by rewrite fmap_id.
+Qed.
+Obligation 2.
+  extensionality st.
+  rewrite /StateT_ap.
+  set f := (X in join (fmap X _)).
+  set g := (X in fmap f (join (fmap X _))).
+  set h := (X in fmap g (join (fmap X _))).
+  set i := (X in join (fmap X (u st))).
+  rewrite -!join_fmap_fmap_x !fmap_comp_x fmap_pure_x
+          join_pure_x -join_fmap_join_x.
+  f_equal; rewrite !fmap_comp_x; f_equal.
+  extensionality u'.
+  case: u' => f' st'.
+  rewrite /i -join_fmap_fmap_x.
+  f_equal; rewrite !fmap_comp_x; f_equal.
+  extensionality v'.
+  case: v' => f'' st''.
+  rewrite /f /first !fmap_comp_x; f_equal.
+  extensionality w'.
+  case: w' => f''' st'''.
+  by rewrite /funcomp.
+Qed.
+Obligation 3.
+  extensionality st.
+  by rewrite /StateT_ap fmap_pure_x join_pure_x fmap_pure_x.
+Qed.
+Obligation 4.
+  extensionality st.
+  rewrite /StateT_ap fmap_pure_x.
+  set f := (X in join (fmap X _)).
+  set g := (X in _ = join (pure (fmap X _))).
+  rewrite join_pure_x.
+  recomp; f_equal.
+  extensionality z.
+  have H1 : pure \o g = f.
+    rewrite /f /g /funcomp.
+    extensionality x.
+    case: x => f' st'.
+    by rewrite fmap_pure_x.
+  by rewrite -H1 /funcomp -fmap_comp_x join_fmap_pure_x.
+Qed.
+Obligation 5.
+  move=> x.
+  extensionality st.
+  rewrite /StateT_ap fmap_pure_x join_pure_x.
+  f_equal.
+Qed.
 
-Definition forM_ `{Monad m} {A B} (l : list A) (f : A -> m B) : m unit :=
-  mapM_ f l.
+Definition StateT_join `{Monad m} {s a : Set} (x : StateT s m (StateT s m a)) :
+  StateT s m a := join \o fmap (curry apply) \o x.
 
-Definition foldM `{Monad m} {A B}
-  (f : A -> B -> m A) (s : A) (l : list B) : m A :=
-  let fix go xs z :=
-      match xs with
-        | nil => pure z
-        | cons y ys => f z y >>= go ys
-      end in
-  go l s.
+Program Instance StateT_Monad `{Monad m} {s : Set} : Monad (StateT s m) := {
+  join := @StateT_join m _ s
+}.
+Obligation 1.
+  move=> f.
+  extensionality st.
+Admitted.
+(*   rewrite /StateT_join /= -!ap_fmap -ap_comp !ap_homo *)
+(*           curry_apply_first !ap_fmap -join_fmap_fmap_x *)
+(*           -join_fmap_join_x fmap_comp_x. *)
+(*   f_equal. *)
+(*   rewrite fmap_comp_x. *)
+(*   f_equal. *)
+(*   extensionality y. *)
+(*   by case: y => f' st'. *)
+(* Qed. *)
+Obligation 2.
+  move=> f.
+  extensionality st.
+  rewrite /StateT_join /= fmap_comp_x /curry /apply /first.
+  set h := (X in fmap X _).
+  replace h with (@pure m _ (a * s)%type); last first.
+    extensionality z.
+    by case: z.
+  by rewrite join_fmap_pure_x.
+Qed.
+Obligation 3.
+  move=> f.
+  extensionality st.
+  by rewrite /StateT_join /= fmap_pure_x join_pure_x.
+Qed.
+Obligation 4.
+  move=> x.
+  extensionality st.
+  rewrite /StateT_join /= -join_fmap_fmap_x.
+  f_equal; rewrite !fmap_comp_x; f_equal.
+  extensionality y.
+  by case: y.
+Qed.
 
-Definition forFoldM `{Monad m} {A B}
-  (s : A) (l : list B) (f : A -> B -> m A) : m A := foldM f s l.
-
-Definition foldrM `{Monad m} {A B}
-  (f : B -> A -> m A) (s : A) (l : list B) : m A :=
-  let fix go xs z :=
-      match xs with
-        | nil => pure z
-        | cons y ys => go ys z >>= f y
-      end in
-  go l s.
-
-Definition forFoldrM `{Monad m} {A B}
-  (s : A) (l : list B) (f : B -> A -> m A) : m A := foldrM f s l.
-
-Fixpoint concat {A} (l : list (list A)) : list A :=
-  match l with
-  | nil => nil
-  | cons x xs => app x (concat xs)
-  end.
-
-Definition concatMapM `{Monad m} {A B}
-  (f : A -> m (list B)) (l : list A) : m (list B) :=
-  fmap (concat) (mapM f l).
+Definition lift `{Monad m} {s} `(x : m a) : StateT s m a :=
+  fun st => (fun z => (z, st)) <$> x.
