Blocks.v
@@ -35,34 +35,38 @@ Definition OpId := nat.
 (* The [OpInfo] structure is a collection of functions that allow us to
    determine information about each operation coming from the caller's
    side. *)
-Record OpInfo (accType opType1 opType2 : Set) := {
+Record OpInfo `{Monad m} (opType1 opType2 : Set) := {
   opKind      : opType1 -> OpKind;
   opRefs      : opType1 -> seq VarInfo;
-  moveOp      : PhysReg -> PhysReg -> accType -> seq opType2 * accType;
-  swapOp      : PhysReg -> PhysReg -> accType -> seq opType2 * accType;
-  saveOp      : PhysReg -> option VarId -> accType -> seq opType2 * accType;
-  restoreOp   : option VarId -> PhysReg -> accType -> seq opType2 * accType;
+  moveOp      : PhysReg -> PhysReg -> m (seq opType2);
+  swapOp      : PhysReg -> PhysReg -> m (seq opType2);
+  saveOp      : PhysReg -> option VarId -> m (seq opType2);
+  restoreOp   : option VarId -> PhysReg -> m (seq opType2);
   applyAllocs : opType1 -> seq (VarId * PhysReg) -> seq opType2;
   showOp      : opType1 -> string
 }.
 
 Definition BlockId := nat.
 
-Record BlockInfo (blockType1 blockType2 opType1 opType2 : Set) := {
+Record BlockInfo `{Monad m} (blockType1 blockType2 opType1 opType2 : Set) := {
   blockId           : blockType1 -> BlockId;
   blockSuccessors   : blockType1 -> seq BlockId;
-  splitCriticalEdge : blockType1 -> blockType1 -> blockType1 * blockType1;
-  blockOps          : blockType1 -> (seq opType1 * seq opType1 * seq opType1);
-  setBlockOps       : blockType1 -> seq opType2 -> seq opType2 -> seq opType2
-                        -> blockType2
+  splitCriticalEdge : blockType1 -> blockType1
+                        -> m (blockType1 * blockType1)%type;
+
+  blockOps    : blockType1 -> (seq opType1 * seq opType1 * seq opType1);
+  setBlockOps : blockType1 -> seq opType2 -> seq opType2 -> seq opType2
+                  -> blockType2
 }.
 
 Close Scope string_scope.
 
-Variables blockType1 blockType2 opType1 opType2 accType : Set.
+Variables blockType1 blockType2 opType1 opType2 : Set.
+Variables mType : Set -> Set.
+Context `{mDict : Monad mType}.
 
 Variable binfo : BlockInfo blockType1 blockType2 opType1 opType2.
-Variable oinfo : OpInfo accType opType1 opType2.
+Variable oinfo : OpInfo opType1 opType2.
 
 Definition allBlockOps (block : blockType1) : seq opType1 :=
   let: (a, b, c) := blockOps binfo block in a ++ b ++ c.
