Resolve.v
@@ -18,10 +18,12 @@ Section Resolve.
 Variable maxReg : nat.          (* max number of registers *)
 Definition PhysReg : predArgType := 'I_maxReg.
 
-Variables blockType1 blockType2 opType1 opType2 accType : Set.
+Variables blockType1 blockType2 opType1 opType2 : Set.
+Variables mType : Set -> Set.
+Context `{mDict : Monad mType}.
 
 Variable binfo : BlockInfo blockType1 blockType2 opType1 opType2.
-Variable oinfo : OpInfo maxReg accType opType1 opType2.
+Variable oinfo : OpInfo maxReg opType1 opType2.
 
 Record Allocation := {
   intId  : nat;
